@prefix liso: <http://purl.imsglobal.org/vocab/lis/v2/outcomes#> .
@prefix owl: <http://www.w3.org/2002/07/owl#> .
@prefix rdf: <http://www.w3.org/1999/02/22-rdf-syntax-ns#> .
@prefix rdfs: <http://www.w3.org/2000/01/rdf-schema#> .
@prefix xsd: <http://www.w3.org/2001/XMLSchema#> .
@prefix bind: <http://purl.org/semantictools/v1/vocab/bind#> .

<http://purl.imsglobal.org/vocab/lis/v2/outcomes#> a owl:Ontology  ;
  rdfs:label "LIS Outcomes" ;
  a bind:TargetNamespace ;
  bind:suggestedPrefix "liso" .

liso:Result rdf:type owl:Class;
  rdfs:subClassOf 
  [ a owl:Restriction ;
    owl:onProperty      liso:resultScore;
    rdfs:comment "The score that the Learner received for engaging in some activity or submitting an assignment."
  ] ; 
  rdfs:comment "A container that holds the result of some scorable activity or assignment." .

liso:Score rdf:type owl:Class ; 
  rdfs:comment "The score that a learner has received for engaging in some activity or submitting an assignment." .

liso:resultScore rdf:type owl:FunctionalProperty ;
  rdfs:domain liso:Result ;
  rdfs:range liso:Score ;
  rdfs:comment "The score that the Learner received for engaging in some activity or submitting an assignment." .

